examples/MemCorrect.v
@@ -2,7 +2,7 @@ Require Import Ascii Bool String List.
 Require Import Lib.CommonTactics Lib.ilist Lib.Word Lib.Struct Lib.StringBound.
 Require Import Lts.Syntax Lts.Semantics Lts.Equiv Lts.Tactics Lts.Specialize.
 Require Import Ex.Msi Ex.MemTypes Ex.Fifo Ex.RegFile Ex.L1Cache Ex.ChildParent Ex.MemDir.
-Require Import Ex.SC Ex.MemAtomic Ex.MemCache.
+Require Import Ex.SC Ex.MemAtomic Ex.MemCache ParametricSyntax Lib.Indexer.
 
 Set Implicit Arguments.
 
@@ -18,9 +18,9 @@ Section MemCorrect.
   Definition memAtomic := memAtomic (L1Cache.AddrBits IdxBits TagBits LgNumDatas LgDataBytes)
                                     LgDataBytes n.
 
-  Lemma memCache_refines_memAtomic: memCache <<== memAtomic.
+  Lemma memCache_refines_memAtomic: makeModule memCache <<== memAtomic.
   Proof.
-    ktrans nmemCache.
+    ktrans (makeModule nmemCache).
     - admit. (* joonwonc TODO *)
     - admit. (* vmurali TODO *)
   Qed.
